feat: improve printing of bottleneck extended-nats

WeightedNetKAT/Examples/Example02.lean
@@ -8,9 +8,9 @@ def p {𝒮 : Type} : Policy[Fields,𝒮] := wnk_policy {
   | dst = H₃ ↦ pt ← 3 ⨁ pt ← 5
   | dst = H₂ ↦ pt ← 2 ⨁ pt ← 5
 }
-def l {𝒮 : Type} : Policy[Fields,𝒮] := wnk_policy {
+def l {𝒮 : Type} [OfNat 𝒮 2] : Policy[Fields,𝒮] := wnk_policy {
   match
-  | pt = 2 ↦ sw ← S₂ ; pt ← 1
+  | pt = 2 ↦ 2 ⨀ sw ← S₂ ; pt ← 1
   | pt = 3 ↦ sw ← S₃ ; pt ← 1
   | pt = 5 ↦ sw ← S₅ ; pt ← 1
 }
@@ -19,12 +19,25 @@ def l {𝒮 : Type} : Policy[Fields,𝒮] := wnk_policy {
 info: {([{dst↦4,pt↦2,sw↦0}, {dst↦4,pt↦0,sw↦0}], 3),
  ([{dst↦4,pt↦3,sw↦0}, {dst↦4,pt↦0,sw↦0}], 3),
  ([{dst↦4,pt↦5,sw↦0}, {dst↦4,pt↦0,sw↦0}], 3),
- ([{dst↦4,pt↦2,sw↦2}, {dst↦4,pt↦1,sw↦2}, {dst↦4,pt↦0,sw↦0}], 3),
- ([{dst↦4,pt↦3,sw↦2}, {dst↦4,pt↦1,sw↦2}, {dst↦4,pt↦0,sw↦0}], 3),
- ([{dst↦4,pt↦5,sw↦2}, {dst↦4,pt↦1,sw↦2}, {dst↦4,pt↦0,sw↦0}], 3)}
+ ([{dst↦4,pt↦2,sw↦2}, {dst↦4,pt↦1,sw↦2}, {dst↦4,pt↦0,sw↦0}], 2),
+ ([{dst↦4,pt↦3,sw↦2}, {dst↦4,pt↦1,sw↦2}, {dst↦4,pt↦0,sw↦0}], 2),
+ ([{dst↦4,pt↦5,sw↦2}, {dst↦4,pt↦1,sw↦2}, {dst↦4,pt↦0,sw↦0}], 2)}
 -/
 #guard_msgs in
 #wnk_eval[Bottleneck Secutiy₄, 2, [pk[dst ↦ H₄]]] {
+  dst = H₄;   dup; (~p; ~l; dup)*; ~p;   true
+}
+
+/--
+info: {([{dst↦4,pt↦2,sw↦0}, {dst↦4,pt↦0,sw↦0}], ⊤),
+ ([{dst↦4,pt↦3,sw↦0}, {dst↦4,pt↦0,sw↦0}], ⊤),
+ ([{dst↦4,pt↦5,sw↦0}, {dst↦4,pt↦0,sw↦0}], ⊤),
+ ([{dst↦4,pt↦2,sw↦2}, {dst↦4,pt↦1,sw↦2}, {dst↦4,pt↦0,sw↦0}], 2),
+ ([{dst↦4,pt↦3,sw↦2}, {dst↦4,pt↦1,sw↦2}, {dst↦4,pt↦0,sw↦0}], 2),
+ ([{dst↦4,pt↦5,sw↦2}, {dst↦4,pt↦1,sw↦2}, {dst↦4,pt↦0,sw↦0}], 2)}
+-/
+#guard_msgs in
+#wnk_eval[Bottleneck ℕ∞, 2, [pk[dst ↦ H₄]]] {
   dst = H₄;   dup; (~p; ~l; dup)*; ~p;   true
 }
 
@@ -35,10 +48,10 @@ def p' {𝒮 : Type} : Policy[Fields,𝒮] := wnk_policy {
   drop
 }
 example (𝒮) : p (𝒮:=𝒮) = p' := by rfl
-def l' {𝒮 : Type} : Policy[Fields,𝒮] := wnk_policy {
-  if pt = 2 then sw ← S₂ ; pt ← 1 else
+def l' {𝒮 : Type} [OfNat 𝒮 2] : Policy[Fields,𝒮] := wnk_policy {
+  if pt = 2 then 2 ⨀ sw ← S₂ ; pt ← 1 else
   if pt = 3 then sw ← S₃ ; pt ← 1 else
   if pt = 5 then sw ← S₅ ; pt ← 1 else
   drop
 }
-example (𝒮) : l (𝒮:=𝒮) = l' := by rfl
+example {𝒮} [OfNat 𝒮 2] : l (𝒮:=𝒮) = l' := by rfl
