WeightedNetKAT/Examples/Example00.lean
@@ -5,3 +5,11 @@ open Fields
 /-- info: {([{dst↦0,pt↦3,sw↦0}], 3), ([{dst↦0,pt↦4,sw↦0}], 2)} -/
 #guard_msgs in
 #wnk_eval[Bottleneck Secutiy₄,1] { pt ← 3 ⨁ 2 ⨀ pt ← 4 }
+
+/-- info: {([{dst↦0,pt↦3,sw↦0}], ⊤), ([{dst↦0,pt↦4,sw↦0}], 2)} -/
+#guard_msgs in
+#wnk_eval[Bottleneck ℕ∞,1] { pt ← 3 ⨁ 2 ⨀ pt ← 4 }
+
+/-- info: {([{dst↦0,pt↦3,sw↦0}], ⊤), ([{dst↦0,pt↦4,sw↦0}], 2)} -/
+#guard_msgs in
+#wnk_eval[Bottleneck EENat,1] { pt ← 3 ⨁ 2 ⨀ pt ← 4 }
